working eq test of super simple avx addition

src/Assembly/TestVector/step_kernel.s
@@ -1,0 +1,165 @@
+	.macosx_version_min 10, 13
+	.section	__TEXT,__text,regular,pure_instructions
+	.section	__TEXT,__const
+	.p2align	5, 0x0                          ## -- Begin function simple_crypto_step___un_3C_uni_3E_un_3C_uni_3E_uni
+LCPI0_0:
+	.long	0                               ## 0x0
+	.long	4                               ## 0x4
+	.long	8                               ## 0x8
+	.long	12                              ## 0xc
+	.long	0                               ## 0x0
+	.long	4                               ## 0x4
+	.long	8                               ## 0x8
+	.long	12                              ## 0xc
+LCPI0_1:
+	.long	0                               ## 0x0
+	.long	1                               ## 0x1
+	.long	2                               ## 0x2
+	.long	3                               ## 0x3
+	.long	4                               ## 0x4
+	.long	5                               ## 0x5
+	.long	6                               ## 0x6
+	.long	7                               ## 0x7
+	.section	__TEXT,__literal16,16byte_literals
+	.p2align	4, 0x0
+LCPI0_2:
+	.long	0                               ## 0x0
+	.long	4                               ## 0x4
+	.long	8                               ## 0x8
+	.long	12                              ## 0xc
+	.section	__TEXT,__text,regular,pure_instructions
+	.globl	_simple_crypto_step___un_3C_uni_3E_un_3C_uni_3E_uni
+	.p2align	4
+_simple_crypto_step___un_3C_uni_3E_un_3C_uni_3E_uni: ## @simple_crypto_step___un_3C_uni_3E_un_3C_uni_3E_uni
+## %bb.0:
+                                        ## kill: def $edx killed $edx def $rdx
+	leal	7(%rdx), %eax
+	testl	%edx, %edx
+	cmovnsl	%edx, %eax
+	andl	$-8, %eax
+	jle	LBB0_1
+## %bb.2:
+	vpcmpeqd	%ymm1, %ymm1, %ymm1
+	vbroadcasti128	LCPI0_2(%rip), %ymm2    ## ymm2 = [0,4,8,12,0,4,8,12]
+                                        ## ymm2 = mem[0,1,0,1]
+	vpxor	%xmm0, %xmm0, %xmm0
+	vpgatherdd	%ymm1, (%rsi,%ymm2), %ymm0
+	movl	%eax, %ecx
+	xorl	%eax, %eax
+	.p2align	4
+LBB0_3:                                 ## =>This Inner Loop Header: Depth=1
+	vpaddd	(%rdi,%rax,4), %ymm0, %ymm1
+	vmovdqu	%ymm1, (%rdi,%rax,4)
+	addq	$8, %rax
+	cmpq	%rcx, %rax
+	jb	LBB0_3
+## %bb.4:
+	cmpl	%edx, %eax
+	jge	LBB0_6
+LBB0_5:
+	vmovd	%eax, %xmm0
+	vpbroadcastd	%xmm0, %ymm0
+	vpor	LCPI0_1(%rip), %ymm0, %ymm0
+	vmovd	%edx, %xmm1
+	vpbroadcastd	%xmm1, %ymm1
+	vpcmpgtd	%ymm0, %ymm1, %ymm0
+	shll	$2, %eax
+	vbroadcasti128	LCPI0_2(%rip), %ymm1    ## ymm1 = [0,4,8,12,0,4,8,12]
+                                        ## ymm1 = mem[0,1,0,1]
+	vpxor	%xmm2, %xmm2, %xmm2
+	vmovdqa	%ymm0, %ymm3
+	vpgatherdd	%ymm3, (%rsi,%ymm1), %ymm2
+	vmaskmovps	(%rdi,%rax), %ymm0, %ymm1
+	vpaddd	%ymm1, %ymm2, %ymm1
+	vmaskmovps	%ymm1, %ymm0, (%rdi,%rax)
+LBB0_6:
+	vzeroupper
+	retq
+LBB0_1:
+	xorl	%eax, %eax
+	cmpl	%edx, %eax
+	jl	LBB0_5
+	jmp	LBB0_6
+                                        ## -- End function
+	.section	__TEXT,__const
+	.p2align	5, 0x0                          ## -- Begin function simple_crypto_step
+LCPI1_0:
+	.long	0                               ## 0x0
+	.long	4                               ## 0x4
+	.long	8                               ## 0x8
+	.long	12                              ## 0xc
+	.long	0                               ## 0x0
+	.long	4                               ## 0x4
+	.long	8                               ## 0x8
+	.long	12                              ## 0xc
+LCPI1_1:
+	.long	0                               ## 0x0
+	.long	1                               ## 0x1
+	.long	2                               ## 0x2
+	.long	3                               ## 0x3
+	.long	4                               ## 0x4
+	.long	5                               ## 0x5
+	.long	6                               ## 0x6
+	.long	7                               ## 0x7
+	.section	__TEXT,__literal16,16byte_literals
+	.p2align	4, 0x0
+LCPI1_2:
+	.long	0                               ## 0x0
+	.long	4                               ## 0x4
+	.long	8                               ## 0x8
+	.long	12                              ## 0xc
+	.section	__TEXT,__text,regular,pure_instructions
+	.globl	_simple_crypto_step
+	.p2align	4
+_simple_crypto_step:                    ## @simple_crypto_step
+## %bb.0:
+                                        ## kill: def $edx killed $edx def $rdx
+	leal	7(%rdx), %eax
+	testl	%edx, %edx
+	cmovnsl	%edx, %eax
+	andl	$-8, %eax
+	jle	LBB1_1
+## %bb.2:
+	vpcmpeqd	%ymm1, %ymm1, %ymm1
+	vbroadcasti128	LCPI1_2(%rip), %ymm2    ## ymm2 = [0,4,8,12,0,4,8,12]
+                                        ## ymm2 = mem[0,1,0,1]
+	vpxor	%xmm0, %xmm0, %xmm0
+	vpgatherdd	%ymm1, (%rsi,%ymm2), %ymm0
+	movl	%eax, %ecx
+	xorl	%eax, %eax
+	.p2align	4
+LBB1_3:                                 ## =>This Inner Loop Header: Depth=1
+	vpaddd	(%rdi,%rax,4), %ymm0, %ymm1
+	vmovdqu	%ymm1, (%rdi,%rax,4)
+	addq	$8, %rax
+	cmpq	%rcx, %rax
+	jb	LBB1_3
+## %bb.4:
+	cmpl	%edx, %eax
+	jge	LBB1_6
+LBB1_5:
+	vmovd	%eax, %xmm0
+	vpbroadcastd	%xmm0, %ymm0
+	vpor	LCPI1_1(%rip), %ymm0, %ymm0
+	vmovd	%edx, %xmm1
+	vpbroadcastd	%xmm1, %ymm1
+	vpcmpgtd	%ymm0, %ymm1, %ymm0
+	shll	$2, %eax
+	vbroadcasti128	LCPI1_2(%rip), %ymm1    ## ymm1 = [0,4,8,12,0,4,8,12]
+                                        ## ymm1 = mem[0,1,0,1]
+	vpxor	%xmm2, %xmm2, %xmm2
+	vmovdqa	%ymm0, %ymm3
+	vpgatherdd	%ymm3, (%rsi,%ymm1), %ymm2
+	vmaskmovps	(%rdi,%rax), %ymm0, %ymm1
+	vpaddd	%ymm1, %ymm2, %ymm1
+	vmaskmovps	%ymm1, %ymm0, (%rdi,%rax)
+LBB1_6:
+	vzeroupper
+	retq
+LBB1_1:
+	xorl	%eax, %eax
+	cmpl	%edx, %eax
+	jl	LBB1_5
+	jmp	LBB1_6
+                                        ## -- End function
+.subsections_via_symbols
